IcTheory.lean
@@ -1,1 +1,4 @@
 import IcTheory.Basics
+import IcTheory.Compression
+import IcTheory.Computability
+import IcTheory.Sanity
